funky fix

src/Init/Control/Option.lean
@@ -104,7 +104,7 @@ Handles failures by treating them as exceptions of type `Unit`.
   let some a ← x | handle ⟨⟩
   pure <| some a
 
-instance : MonadExceptOf PUnit (OptionT m) where
+instance (priority := low) : MonadExceptOf PUnit (OptionT m) where
   throw    := fun _ => OptionT.fail
   tryCatch := OptionT.tryCatch
 
